Clean up files and test report, delete

Rope.dfy
@@ -1,52 +1,296 @@
 include "Utils.dfy"
 
-module BinaryTree {
-  import opened Utils
-  trait Node
-  {
-    var height: nat;
+module Rope {
+    import Utils
 
-    function length(): nat
-      reads this
-      decreases this.height
-  }
+    class Node {
+        ghost var Contents: string;
+        ghost var Repr: set<Node>;
 
-  class NTNode extends Node
-  {
-    var leftLen: nat;
-    var left: Node?;
-    var right: Node?;
+        var data: string;
+        var weight: nat;
+        var left: Node?;
+        var right: Node?;
 
-    constructor (left: Node, right: Node)
-      ensures this.leftLen == left.length()
-      ensures this.height > left.height
-      ensures this.height > right.height
+        ghost predicate Valid() 
+            reads this, Repr
+            ensures Valid() ==> this in Repr
+        {
+            this in Repr &&
+            (left != null ==> 
+                left in Repr &&
+                left.Repr < Repr && this !in left.Repr &&
+                left.Valid() &&
+                (forall child :: child in left.Repr ==> child.weight <= weight)) &&
+            (right != null ==> 
+                right in Repr &&
+                right.Repr < Repr && this !in right.Repr &&
+                right.Valid()) &&
+            (left == null && right == null ==>
+                Repr == {this} &&
+                Contents == data &&
+                weight == |data| &&
+                data != "") &&
+            (left != null && right == null ==>
+                Repr == {this} + left.Repr &&
+                Contents == left.Contents &&
+                weight == |left.Contents| &&
+                data == "") &&
+            (left == null && right != null ==>
+                Repr == {this} + right.Repr &&
+                Contents == right.Contents &&
+                weight == 0 &&
+                data == "") &&
+            (left != null && right != null ==>
+                Repr == {this} + left.Repr + right.Repr &&
+                left.Repr !! right.Repr &&
+                Contents == left.Contents + right.Contents &&
+                weight == |left.Contents| &&
+                data == "") 
+        }
+
+        static lemma contentSizeGtZero(n: Node)
+            requires n.Valid()
+            ensures |n.Contents| > 0
+            decreases n.Repr
+        {}
+
+        function getWeightsOfAllRightChildren(): nat
+            reads right, Repr
+            requires Valid()
+            decreases Repr
+        {
+            if right == null then 0 else right.weight + right.getWeightsOfAllRightChildren()
+        } 
+
+        // constructor for creating a terminal node
+        constructor Terminal(x: string)
+            requires x != ""
+            ensures Valid() && fresh(Repr) && left == null && right == null && data == x
+        { 
+            data := x;
+            weight := |x|;
+            left := null;
+            right := null;
+            Contents := x;
+            Repr := {this};
+        }   
+
+        predicate isTerminal(n: Node)
+            reads n, n.left, n.right
+        { n.left == null && n.right == null }
+
+        // constructor for creating a non-terminal node
+        constructor NonTerminal(nLeft: Node, nRight: Node)
+            requires nLeft.Valid() && nRight.Valid() && nLeft.Repr !! nRight.Repr
+            ensures Valid() && left == nLeft && right == nRight && fresh(Repr - nLeft.Repr - nRight.Repr)
+        { 
+            left := nLeft;
+            right := nRight;
+            data := "";
+
+            var nTemp := nLeft;
+            var w := 0;
+            ghost var nodesTraversed : set<Node> := {};
+
+            while (nTemp.right != null)
+                invariant nTemp != null
+                invariant nTemp.Valid()
+                invariant forall node :: node in nodesTraversed ==> node.weight <= w
+                invariant nodesTraversed == nLeft.Repr - nTemp.Repr
+                invariant nTemp.right == null ==> w + nTemp.weight == |nLeft.Contents|
+                invariant nTemp.right != null ==> w + nTemp.weight + |nTemp.right.Contents| == |nLeft.Contents| 
+                decreases nTemp.Repr
+            {
+                w := w + nTemp.weight;
+                assert w >= 0;
+                if (nTemp.left != null) {
+                    nodesTraversed := nodesTraversed + nTemp.left.Repr + {nTemp};
+                } else {
+                    nodesTraversed := nodesTraversed + {nTemp};
+                }
+                nTemp := nTemp.right;
+            }
+            w := w + nTemp.weight;
+            if (nTemp.left != null) {
+                nodesTraversed := nodesTraversed + nTemp.left.Repr + {nTemp};
+            } else {
+                nodesTraversed := nodesTraversed + {nTemp};
+            }
+            weight := w;
+
+            Contents := nLeft.Contents + nRight.Contents;
+            Repr := {this} + nLeft.Repr + nRight.Repr;
+        }   
+
+        method getCharAtIndex(index: nat) returns (nTemp: Node, i: nat, c: char)
+            requires Valid() && 0 <= index < |Contents|
+            ensures c == Contents[index]
+            ensures 0 <= i < |nTemp.data|
+            ensures nTemp.Valid() && nTemp.data[i] == c
+            ensures nTemp in Repr && isTerminal(nTemp)
+        {
+            nTemp := this;
+            i := index;
+            while (!isTerminal(nTemp)) 
+                invariant nTemp.Valid()
+                invariant 0 <= i < |nTemp.Contents|   
+                invariant nTemp.Contents[i] == Contents[index] 
+                decreases nTemp.Repr
+            {
+                if (i < nTemp.weight) {
+                    nTemp := nTemp.left;
+                } else {
+                    i := i - nTemp.weight;
+                    nTemp := nTemp.right;
+                }
+            }
+            // Have reached the terminal node with index i
+            c := nTemp.data[i];
+        }
+
+
+        method report(i: nat, j: nat) returns (s: string)
+            requires 0 <= i <= j <= |this.Contents|
+            requires Valid()
+            ensures s == this.Contents[i..j]
+            decreases Repr
+        {
+            if i == j {
+                s := "";
+            } else {
+                if this.left == null && this.right == null {
+                    s := data[i..j];
+                    // strange: removing this assert fails the postcondition.
+                    assert s == this.Contents[i..j];
+                } else {
+                    if (j <= this.weight) {
+                        var s' := this.left.report(i, j);
+                        s := s';
+                    } else if (this.weight <= i) {
+                        var s' := this.right.report(i - this.weight, j - this.weight);
+                        s := s';
+                        // strange: removing this assert fails the postcondition.
+                        assert s == this.Contents[i..j];
+                    } else {
+                        assert i <= this.weight < j;
+                        assert this.weight == |this.left.Contents|;
+                        var s1 := this.left.report(i, this.weight);
+                        var s2 := this.right.report(0, j - this.weight);
+                        s := s1 + s2;
+                    }
+                }
+            }
+        }
+
+    }
+    // End of Node Class
+
+
+    method concat(n1: Node?, n2: Node?) returns (n: Node?) 
+        requires (n1 != null) ==> n1.Valid()
+        requires (n2 != null) ==> n2.Valid()
+        requires (n1 != null && n2 != null) ==> (n1.Repr !! n2.Repr)
+        ensures (n1 != null || n2 != null) ==> n != null && n.Valid()
+        ensures (n1 == null && n2 == null) ==> n == null
+        ensures (n1 == null && n2 != null) ==> n == n2 && n != null && n.Valid() && n.Contents == n2.Contents
+        ensures (n1 != null && n2 == null) ==> n == n1 && n != null && n.Valid() && n.Contents == n1.Contents
+        ensures (n1 != null && n2 != null) ==> (n != null && n.Valid() && n.left == n1 && n.right == n2 && 
+                                                n.Contents == n1.Contents + n2.Contents && fresh(n.Repr - n1.Repr - n2.Repr))
     {
-      this.left := left;
-      this.right := right;
-      this.leftLen := left.length();
-      this.height := max(left.height, right.height) + 1;
+        if (n1 == null) {
+            n := n2;
+        } else if (n2 == null) {
+            n := n1;
+        } else {
+            n := new Node.NonTerminal(n1, n2);
+        } 
+    } 
+
+
+    /**
+        Dafny needs help to guess that in our definition, every rope must
+        have non-empty Contents, otherwise it is represented by [null].
+
+        The lemma contentSizeGtZero(n) is thus important to prove the
+        postcondition of this method, in the two places where the lemma is
+        invoked.
+     */
+    method split(n: Node, index: nat) returns (n1: Node?, n2: Node?) 
+        requires n.Valid() && 0 <= index <= |n.Contents|
+        ensures index == 0 ==> (n1 == null && n2 != null && n2.Valid() && n2.Contents == n.Contents && fresh(n2.Repr - n.Repr))
+        ensures index == |n.Contents| ==> (n2 == null && n1 != null && n1.Valid() && n1.Contents == n.Contents && fresh(n1.Repr - n.Repr))
+        ensures 0 < index < |n.Contents| ==> (n1 != null && n1.Valid() && n2 != null && n2.Valid() && 
+                                                n1.Contents == n.Contents[..index] && n2.Contents == n.Contents[index..] &&
+                                                n1.Repr !! n2.Repr && fresh(n1.Repr - n.Repr) && fresh(n2.Repr - n.Repr))
+        decreases n.Repr
+    {
+        if (index == 0) {
+            n1 := null;
+            n2 := n;
+            Node.contentSizeGtZero(n);
+            // assert index != |n.Contents|;
+        } else if (index < n.weight) {
+            if (n.left != null) {
+                var s1, s2 := split(n.left, index);
+                n1 := s1;
+                n2 := concat(s2, n.right);
+            } else {
+                // terminal node
+                if (index == 0) {
+                    n1 := null;
+                    n2 := n;
+                } else {
+                    n1 := new Node.Terminal(n.data[..index]);
+                    n2 := new Node.Terminal(n.data[index..]);
+                }
+            }
+        } else if (index > n.weight) {
+            var s1, s2 := split(n.right, index - n.weight);
+            n1 := concat(n.left, s1);
+            n2 := s2;
+        } else {
+            // since [n.weight == index != 0], it means that [n] cannot be a
+            // non-terminal node with [left == null].
+            if (n.left != null && n.right == null) {
+                n1 := n.left;
+                n2 := null;
+            } else if (n.left != null && n.right != null) {
+                n.contentSizeGtZero(n.right);
+                // assert index != |n.Contents|;
+                n1 := n.left;
+                n2 := n.right;
+            } else {
+                assert n.left == null && n.right == null;
+                n1 := n;
+                n2 := null;
+            }
+        }
     }
 
-    function length(): nat
-      reads this
+    method insert(n1: Node, n2: Node, index: nat) returns (n: Node)
+        requires n1.Valid() && n2.Valid() && n1.Repr !! n2.Repr
+        requires 0 <= index < |n1.Contents|
+        ensures n.Valid() && n.Contents == n1.Contents[..index] + n2.Contents + n1.Contents[index..] && fresh(n.Repr - n1.Repr - n2.Repr)
     {
-      this.leftLen + (if this.right == null then 0 else this.right.length())
-    }
-  }
-
-  class TNode extends Node
-  {
-    var str: string;
-
-    constructor(str: string)
-    {
-      this.str := str;
-      this.height := 1;
+        var n1BeforeIndex, n1AfterIndex := split(n1, index);
+        var firstPart := concat(n1BeforeIndex, n2);
+        n := concat(firstPart, n1AfterIndex);
     }
 
-    function length(): nat
-      reads this
-    { |this.str| }
-  }
+    method delete(n: Node, i: nat, j: nat) returns (m: Node?)
+        requires n.Valid()
+        requires 0 <= i < j <= |n.Contents|
+        ensures (i == 0 && j == |n.Contents|) <==> m == null
+        ensures m != null ==>
+            m.Valid() &&
+            m.Contents == n.Contents[..i] + n.Contents[j..] &&
+            fresh(m.Repr - n.Repr)
+        
+    {
+        var l1, l2 := split(n, i);
+        var r1, r2 := split(l2, j - i);
+        m := concat(l1, r2);
+    }
 }
+// End of Rope Module
